theories/simulation/simulation.v
@@ -8,13 +8,19 @@ Import bi.
 (* parameterized over value relation that restricts values passed to functions *)
 Class simulirisG (PROP : bi) (Λ : language) := {
   (* state interpretation *)
-  state_interp : prog Λ → state Λ → prog Λ → state Λ → PROP;
+  state_interp : prog Λ → state Λ → prog Λ → state Λ → list (expr Λ) → PROP;
+  state_interp_pure_prim_step P_t σ_t P_s σ_s e_s T π e_s':
+    T !! π = Some e_s →
+    (∀ σ_s, prim_step P_s e_s σ_s e_s' σ_s []) →
+    state_interp P_t σ_t P_s σ_s T -∗
+    state_interp P_t σ_t P_s σ_s (<[π:=e_s']>T)
+
 }.
 #[global]
 Hint Mode simulirisG + - : typeclass_instances.
 
 Definition progs_are {Λ PROP} `{simulirisG PROP Λ} (P_t P_s : prog Λ) : PROP :=
-  (□ ∀ P_t' P_s' σ_t σ_s, state_interp P_t' σ_t P_s' σ_s → ⌜P_t' = P_t⌝ ∧ ⌜P_s' = P_s⌝)%I.
+  (□ ∀ P_t' P_s' σ_t σ_s T_s, state_interp P_t' σ_t P_s' σ_s T_s → ⌜P_t' = P_t⌝ ∧ ⌜P_s' = P_s⌝)%I.
 #[global]
 Hint Mode progs_are - - - + + : typeclass_instances.
 Typeclasses Opaque progs_are.
@@ -27,33 +33,36 @@ Proof. rewrite /progs_are; apply _. Qed.
 (** Typeclass for the simulation relation so we can use the definitions with
    greatest+least fp (stuttering) or just greatest fp (no stuttering). *)
 Class Sim {PROP : bi} {Λ : language} (s : simulirisG PROP Λ) :=
-  sim : (val Λ → val Λ → PROP) → (val Λ → val Λ → PROP) → expr Λ → expr Λ → PROP.
+  sim : (val Λ → val Λ → PROP) → (val Λ → val Λ → PROP) → thread_id → expr Λ → expr Λ → PROP.
 #[global]
 Hint Mode Sim - - - : typeclass_instances.
 
 Class SimE {PROP : bi} {Λ : language} (s : simulirisG PROP Λ) :=
-  sim_expr : (val Λ → val Λ → PROP) → (expr Λ → expr Λ → PROP) → expr Λ → expr Λ → PROP.
+  sim_expr : (val Λ → val Λ → PROP) → (expr Λ → expr Λ → PROP) → thread_id → expr Λ → expr Λ → PROP.
 #[global]
 Hint Mode SimE - - - : typeclass_instances.
 
 (* FIXME what are good levels for et, es? *)
-Notation "et '⪯{' Ω '}' es {{ Φ }}" := (sim Ω Φ et es) (at level 40, Φ at level 200,
-  format "et  '⪯{' Ω '}'  es  {{  Φ  }}") : bi_scope.
+Notation "et '⪯{' π , Ω '}' es {{ Φ }}" := (sim Ω Φ π et es) (at level 40, Φ at level 200,
+  format "et  '⪯{' π ,  Ω '}'  es  {{  Φ  }}") : bi_scope.
 
 (* FIXME: the notation with binder doesn't work; left-factoring seems to fail.
 Notation "et  '⪯'  es  {{  v_t  v_s ,  P  }}" := (sim et es (λ v_t v_s, P)) (at level 40, v_t, v_s at level 200, P at level 200) : bi_scope. *)
 
 
 (* TODO: different symbols (no brackets) for expr thing *)
-Notation "et '⪯{' Ω '}' es [{ Φ }]" := (sim_expr Ω Φ et es) (at level 40, Φ at level 200,
-  format "et  '⪯{' Ω '}'  es  [{  Φ  }]") : bi_scope.
+Notation "et '⪯{' π , Ω '}' es [{ Φ }]" := (sim_expr Ω Φ π et es) (at level 40, Φ at level 200,
+  format "et  '⪯{' π ,  Ω '}'  es  [{  Φ  }]") : bi_scope.
 
 
 
 
-(* discrete OFE instance for expr *)
+(* discrete OFE instance for expr and thread_id *)
 Definition exprO {Λ : language} := leibnizO (expr Λ).
 Instance expr_equiv {Λ} : Equiv (expr Λ). apply exprO. Defined.
+
+Definition thread_idO := leibnizO thread_id.
+Instance thread_id_equiv : Equiv thread_id. apply thread_idO. Defined.
 
 (** * SLSLS, Separation Logic Stuttering Local Simulation *)
 Section fix_lang.
@@ -66,9 +75,8 @@ Section fix_lang.
 
   Implicit Types (e_s e_t e: expr Λ).
 
-  Definition sim_ectx `{!Sim s} K_t K_s Φ :=
-    (∀ v_t v_s, Ω v_t v_s -∗ sim Ω Φ (fill K_t (of_val v_t)) (fill K_s (of_val v_s)))%I.
-  Definition sim_expr_ectx `{!SimE s} K_t K_s Φ :=
-    (∀ v_t v_s, Ω v_t v_s -∗ sim_expr Ω Φ (fill K_t (of_val v_t)) (fill K_s (of_val v_s)))%I.
+  Definition sim_ectx `{!Sim s} π K_t K_s Φ :=
+    (∀ v_t v_s, Ω v_t v_s -∗ sim Ω Φ π (fill K_t (of_val v_t)) (fill K_s (of_val v_s)))%I.
+  Definition sim_expr_ectx `{!SimE s} π K_t K_s Φ :=
+    (∀ v_t v_s, Ω v_t v_s -∗ sim_expr Ω Φ π (fill K_t (of_val v_t)) (fill K_s (of_val v_s)))%I.
 End fix_lang.
-
