theories/simulation/lifting.v
@@ -109,26 +109,40 @@ Hint Mode PureExec - - - + - : core.
 Section fix_sim.
   Context {PROP : bi} `{!BiBUpd PROP, !BiAffine PROP, !BiPureForall PROP}.
   Context {Λ : language} {s : simulirisG PROP Λ}.
-  Context (Ω : val Λ → val Λ → PROP).
+  Context (Ω : val Λ → val Λ → PROP) (π : thread_id).
 
   Implicit Types
     (e_s e_t e: expr Λ)
     (P_s P_t P: prog Λ)
     (σ_s σ_t σ : state Λ).
-  Local Notation "et '⪯' es [{ Φ }]" := (et ⪯{Ω} es [{Φ}])%I (at level 40, Φ at level 200) : bi_scope.
+  Local Notation "et '⪯' es [{ Φ }]" := (et ⪯{π, Ω} es [{Φ}])%I (at level 40, Φ at level 200) : bi_scope.
+
+  Lemma state_interp_pure_step P_t σ_t P_s σ_s e_s T e_s' K_s:
+    pure_step e_s e_s' →
+    T !! π = Some (fill K_s e_s) →
+    state_interp (PROP := PROP) P_t σ_t P_s σ_s T -∗
+    state_interp P_t σ_t P_s σ_s (<[π:=fill K_s e_s']>T).
+  Proof.
+    intros [Hsafe Hred] ?. apply: state_interp_pure_prim_step; [done|].
+    intros σ. eapply fill_prim_step.
+    destruct (Hsafe P_s σ) as [?[? [? Hstep]]].
+    by destruct (Hred _ _ _ _ _ Hstep) as [->[-> ->]].
+  Qed.
+
 
   (** Pure reduction *)
   Lemma source_red_lift_pure Ψ m e_s1 e_s2 ϕ :
     PureExec ϕ m e_s1 e_s2 →
-    ϕ → source_red e_s2 Ψ -∗ source_red e_s1 Ψ.
+    ϕ → source_red e_s2 π Ψ -∗ source_red e_s1 π Ψ.
   Proof.
     intros Hp Hϕ. specialize (Hp Hϕ).
     induction Hp as [ e_s2 | n e_s1 e_s2 e_s3 Hstep _ IH]; first done.
     rewrite IH. iIntros "Hs". iApply source_red_step.
-    iIntros (????) "[Hstate %Hnreach]". iModIntro. iExists e_s2, σ_s.
+    iIntros (??????) "[Hstate [% %]]". iModIntro. iExists e_s2, σ_s.
     iFrame.
-    destruct Hstep as [Hred Hdet]. destruct (Hred P_s σ_s) as (e_s' & σ_s' & efs & H).
-    by specialize (Hdet _ _ _ _ _ H) as [-> [-> ->]].
+    destruct (Hstep) as [Hred Hdet]. destruct (Hred P_s σ_s) as (e_s' & σ_s' & efs & Hs).
+    specialize (Hdet _ _ _ _ _ Hs) as [-> [-> ->]].
+    iSplitR; [done|]. by iApply state_interp_pure_step.
   Qed.
 
   Lemma target_red_lift_pure Ψ n e1 e2 ϕ :
@@ -138,23 +152,24 @@ Section fix_sim.
     intros Hp Hϕ. specialize (Hp Hϕ).
     induction Hp as [ e_t2 | n e_t1 e_t2 e_t3 Hstep _ IH]; first done.
     rewrite IH. iIntros "Ht". iApply target_red_step.
-    iIntros (????) "Hstate". iModIntro. iSplitR. { iPureIntro. apply Hstep. }
+    iIntros (?????) "Hstate". iModIntro. iSplitR. { iPureIntro. apply Hstep. }
     iIntros (???) "%". iModIntro. apply Hstep in H as [-> [-> ->]]. by iFrame.
   Qed.
 
   (** Primitive reduction *)
   Lemma sim_lift_prim_step_both e_t e_s Φ:
-    (∀ P_t P_s σ_t σ_s, state_interp P_t σ_t P_s σ_s ∗ ⌜¬ reach_stuck P_s e_s σ_s⌝ ==∗
+    (∀ P_t P_s σ_t σ_s T_s K_s, state_interp P_t σ_t P_s σ_s T_s ∗ ⌜T_s !! π = Some (fill K_s e_s)
+        ∧ pool_safe P_s T_s σ_s⌝ ==∗
       ⌜reducible P_t e_t σ_t⌝ ∗
       ∀ e_t' efs_t σ_t',
         ⌜prim_step P_t e_t σ_t e_t' σ_t' efs_t⌝ ==∗
           ∃ e_s' efs_s σ_s', ⌜prim_step P_s e_s σ_s e_s' σ_s' efs_s⌝ ∗
-            state_interp P_t σ_t' P_s σ_s' ∗ e_t' ⪯{Ω} e_s' [{ Φ }] ∗
-            ([∗ list] e_t0;e_s0 ∈ efs_t;efs_s, e_t0 ⪯ e_s0 [{lift_post Ω}])) -∗
-    e_t ⪯{Ω} e_s [{ Φ }].
+            state_interp P_t σ_t' P_s σ_s' (<[π:=K_s e_s']>T_s ++ efs_s) ∗ e_t' ⪯{π, Ω} e_s' [{ Φ }] ∗
+            ([∗ list] π'↦e_t0;e_s0 ∈ efs_t;efs_s, e_t0 ⪯{length T_s + π', Ω} e_s0 [{lift_post Ω}])) -∗
+    e_t ⪯{π, Ω} e_s [{ Φ }].
   Proof.
     iIntros "Hsim".
-    rewrite sim_expr_unfold. iIntros (????) "[Hstate %]".
+    rewrite sim_expr_unfold. iIntros (??????) "[Hstate [% %]]".
     iMod ("Hsim" with "[$Hstate ]") as "[Hred Hsim]"; first done. iModIntro. iRight; iLeft.
     iFrame. iIntros (e_t' efs_t σ_t') "Hstep".
     iMod ("Hsim" with "Hstep") as (e_s' efs_s σ_s') "(Hs & ? & ? & Hefs)".
@@ -163,49 +178,52 @@ Section fix_sim.
   Qed.
 
   Lemma sim_lift_prim_step_target e_t e_s Φ :
-    (∀ P_t P_s σ_t σ_s, state_interp P_t σ_t P_s σ_s ∗ ⌜¬ reach_stuck P_s e_s σ_s⌝ ==∗
+    (∀ P_t P_s σ_t σ_s T_s K_s, state_interp P_t σ_t P_s σ_s T_s ∗ ⌜T_s !! π = Some (fill K_s e_s)
+        ∧ pool_safe P_s T_s σ_s⌝ ==∗
       ⌜reducible P_t e_t σ_t⌝ ∗
       ∀ e_t' efs_t σ_t',
         ⌜prim_step P_t e_t σ_t e_t' σ_t' efs_t⌝ ==∗
           ⌜efs_t = []⌝ ∗
-          state_interp P_t σ_t' P_s σ_s ∗
-          e_t' ⪯{Ω} e_s [{ Φ }]) -∗
-    e_t ⪯{Ω} e_s [{ Φ }].
+          state_interp P_t σ_t' P_s σ_s T_s ∗
+          e_t' ⪯{π, Ω} e_s [{ Φ }]) -∗
+    e_t ⪯{π, Ω} e_s [{ Φ }].
   Proof.
     iIntros "Ha".
-    iApply sim_step_target. iIntros (????) "[Hstate %Hnreach]".
+    iApply sim_step_target. iIntros (??????) "[Hstate [% %]]".
     iMod ("Ha" with "[$Hstate//]") as "[Hred Hev]". iModIntro. iFrame.
     iIntros (e_t' efs_t σ_t') "Htarget". iMod ("Hev" with "Htarget") as "[Hstate Hev]".
-    iModIntro; iExists e_s, σ_s. iFrame. iPureIntro; constructor.
+    iModIntro; iExists e_s, σ_s. rewrite list_insert_id //. iFrame. iPureIntro; constructor.
   Qed.
 
   Lemma sim_lift_prim_step_source e_t e_s Φ :
-    (∀ P_t P_s σ_t σ_s, state_interp P_t σ_t P_s σ_s ==∗
+    (∀ P_t P_s σ_t σ_s T_s K_s, state_interp P_t σ_t P_s σ_s T_s ∗ ⌜T_s !! π = Some (fill K_s e_s)
+        ∧ pool_safe P_s T_s σ_s⌝ ==∗
       ∃ e_s' σ_s',
         ⌜prim_step P_s e_s σ_s e_s' σ_s' []⌝ ∗
-          state_interp P_t σ_t P_s σ_s' ∗
-          e_t ⪯{Ω} e_s' [{ Φ }]) -∗
-    e_t ⪯{Ω} e_s [{ Φ }].
+          state_interp P_t σ_t P_s σ_s' (<[π := fill K_s e_s']>T_s) ∗
+          e_t ⪯{π, Ω} e_s' [{ Φ }]) -∗
+    e_t ⪯{π, Ω} e_s [{ Φ }].
   Proof.
     iIntros "Hsource". iApply sim_step_source.
-    iIntros (????) "[Hstate %Hnreach]".
-    iMod ("Hsource" with "Hstate") as (e_s' σ_s') "[% Hstate]".
+    iIntros (??????) "[Hstate [% %]]".
+    iMod ("Hsource" with "[$Hstate//]") as (e_s' σ_s') "[% Hstate]".
     iModIntro. iExists e_s', σ_s'. iFrame. iPureIntro.
     econstructor; [done|by econstructor].
   Qed.
 
   (** Head reduction *)
   Lemma sim_lift_head_step_target e_t e_s Φ :
-    (∀ P_t P_s σ_t σ_s, state_interp P_t σ_t P_s σ_s ∗ ⌜¬ reach_stuck P_s e_s σ_s⌝ ==∗
+    (∀ P_t P_s σ_t σ_s T_s K_s, state_interp P_t σ_t P_s σ_s T_s ∗ ⌜T_s !! π = Some (fill K_s e_s)
+        ∧ pool_safe P_s T_s σ_s⌝ ==∗
       ⌜head_reducible P_t e_t σ_t⌝ ∗
       ∀ e_t' efs_t σ_t',
         ⌜head_step P_t e_t σ_t e_t' σ_t' efs_t⌝ ==∗
           ⌜efs_t = []⌝ ∗
-          state_interp P_t σ_t' P_s σ_s ∗
-          e_t' ⪯{Ω} e_s [{ Φ }]) -∗
-    e_t ⪯{Ω} e_s [{ Φ }].
+          state_interp P_t σ_t' P_s σ_s T_s ∗
+          e_t' ⪯{π, Ω} e_s [{ Φ }]) -∗
+    e_t ⪯{π, Ω} e_s [{ Φ }].
   Proof.
-    iIntros "Htarget". iApply sim_lift_prim_step_target. iIntros (????) "[Hstate %Hnreach]".
+    iIntros "Htarget". iApply sim_lift_prim_step_target. iIntros (??????) "[Hstate [% %]]".
     iMod ("Htarget" with "[$Hstate//]") as "(%Hred & Hstep)". iModIntro.
     iSplitR. { iPureIntro. by apply head_prim_reducible. }
     iIntros (e_t' efs_t σ_t') "%Hprim". iApply "Hstep".
@@ -214,29 +232,31 @@ Section fix_sim.
 
   (* for symmetry, in this lemma nothing actually happens *)
   Lemma sim_lift_head_step_source e_t e_s Φ :
-    (∀ P_t P_s σ_t σ_s, state_interp P_t σ_t P_s σ_s ==∗
+    (∀ P_t P_s σ_t σ_s T_s K_s, state_interp P_t σ_t P_s σ_s T_s ∗ ⌜T_s !! π = Some (fill K_s e_s)
+        ∧ pool_safe P_s T_s σ_s⌝ ==∗
       ∃ e_s' σ_s',
         ⌜head_step P_s e_s σ_s e_s' σ_s' []⌝ ∗ |==>
-          (state_interp P_t σ_t P_s σ_s' ∗
-          e_t ⪯{Ω} e_s' [{ Φ }])) -∗
-    e_t ⪯{Ω} e_s [{ Φ }].
+          (state_interp P_t σ_t P_s σ_s' (<[π:= fill K_s e_s']>T_s) ∗
+          e_t ⪯{π, Ω} e_s' [{ Φ }])) -∗
+    e_t ⪯{π, Ω} e_s [{ Φ }].
   Proof.
     iIntros "Hsource". iApply sim_lift_prim_step_source.
-    iIntros (????) "Hstate". iMod ("Hsource" with "Hstate") as (e_s' σ_s') "[% >Hstate]".
+    iIntros (??????) "[Hstate %]". iMod ("Hsource" with "[$Hstate//]") as (e_s' σ_s') "[% >Hstate]".
     iModIntro. iExists e_s', σ_s'. iFrame. iPureIntro. by apply head_prim_step.
   Qed.
 
   Lemma sim_lift_head_step_both e_t e_s Φ:
-    (∀ P_t P_s σ_t σ_s, state_interp P_t σ_t P_s σ_s ∗ ⌜¬ reach_stuck P_s e_s σ_s⌝ ==∗
+    (∀ P_t P_s σ_t σ_s T_s K_s, state_interp P_t σ_t P_s σ_s T_s ∗ ⌜T_s !! π = Some (fill K_s e_s)
+        ∧ pool_safe P_s T_s σ_s⌝ ==∗
       ⌜head_reducible P_t e_t σ_t⌝ ∗
       ∀ e_t' efs_t σ_t',
         ⌜head_step P_t e_t σ_t e_t' σ_t' efs_t⌝ ==∗
           ∃ e_s' efs_s σ_s', ⌜head_step P_s e_s σ_s e_s' σ_s' efs_s⌝ ∗
-          state_interp P_t σ_t' P_s σ_s' ∗ e_t' ⪯{Ω} e_s' [{ Φ }] ∗
-          ([∗ list] e_t0;e_s0 ∈ efs_t;efs_s, e_t0 ⪯ e_s0 [{lift_post Ω}])) -∗
-    e_t ⪯{Ω} e_s [{ Φ }].
+          state_interp P_t σ_t' P_s σ_s' (<[π:=fill K_s e_s']>T_s ++ efs_s) ∗ e_t' ⪯{π, Ω} e_s' [{ Φ }] ∗
+          ([∗ list] π'↦e_t0;e_s0 ∈ efs_t;efs_s, e_t0 ⪯{length T_s + π', Ω} e_s0 [{lift_post Ω}])) -∗
+    e_t ⪯{π, Ω} e_s [{ Φ }].
   Proof.
-    iIntros "Hsim". iApply sim_lift_prim_step_both. iIntros (????) "[Hstate %Hnreach]".
+    iIntros "Hsim". iApply sim_lift_prim_step_both. iIntros (??????) "[Hstate %Hnreach]".
     iMod ("Hsim" with "[$Hstate//]") as "(% & Hstep)".
     iModIntro. iSplitR. { iPureIntro. by eapply head_prim_reducible. }
     iIntros (e_t' efs_t σ_t') "%". iMod ("Hstep" with "[]") as (e_s' efs_s σ_s') "(% & Hstate & Hsim)".
@@ -249,24 +269,26 @@ Section fix_sim.
     (∀ P_s σ_s, SIrreducible ϕ P_s e_s σ_s) →
     ϕ →
     to_val e_s = None →
-    ⊢ source_red e_s Ψ.
+    ⊢ source_red e_s π Ψ.
   Proof.
     intros Hirred Hp Hval. iApply source_red_stuck.
-    iIntros (????) "_ !>". iPureIntro. split; first done.
+    iIntros (?????) "_ !>". iPureIntro. split; first done.
       by intros e' σ' efs Hprim%Hirred.
   Qed.
 
   Lemma source_red_irred_unless ϕ e_s Ψ :
     (∀ P_s σ_s, IrredUnless ϕ P_s e_s σ_s) →
     to_val e_s = None →
-    (⌜ϕ⌝ -∗ source_red e_s Ψ) -∗
-    source_red e_s Ψ.
+    (⌜ϕ⌝ -∗ source_red e_s π Ψ) -∗
+    source_red e_s π Ψ.
   Proof.
     intros Hunless Hval. iIntros "Hs".
     rewrite source_red_eq /flip source_red_unfold /source_red_rec /safe.
-    iIntros (????) "[Hstate %Hnreach]".
+    iIntros (??????) "[Hstate [% %Hnreach]]".
     assert (¬ irreducible P_s e_s σ_s) as Hn.
-    { contradict Hnreach. by apply stuck_reach_stuck. }
+    { unfold pool_safe in Hnreach. contradict Hnreach.
+      apply: pool_reach_stuck_reach_stuck; [|done].
+      apply: fill_reach_stuck. by apply stuck_reach_stuck. }
     apply Hunless in Hn. iMod ("Hs" with "[//] [$Hstate //]") as "Hs"; done.
   Qed.
 
@@ -278,20 +300,22 @@ Section fix_sim.
   Proof.
     intros Hunless Hval. iIntros "Hs".
     rewrite sim_expr_unfold /safe.
-    iIntros (????) "[Hstate %Hnreach]".
+    iIntros (??????) "[Hstate [% %Hnreach]]".
     assert (¬ irreducible P_s e_s σ_s) as Hn.
-    { contradict Hnreach. by apply stuck_reach_stuck. }
+    { unfold pool_safe in Hnreach. contradict Hnreach.
+      apply: pool_reach_stuck_reach_stuck; [|done].
+      apply: fill_reach_stuck. by apply stuck_reach_stuck. }
     apply Hunless in Hn. iMod ("Hs" with "[//] [$Hstate //]") as "Hs"; done.
   Qed.
 
   (** Target eval *)
   Lemma target_red_lift_head_step Ψ e_t :
-    ⊢ (∀ P_s σ_s P_t σ_t, state_interp P_t σ_t P_s σ_s ==∗
+    ⊢ (∀ P_s σ_s P_t σ_t T_s, state_interp P_t σ_t P_s σ_s T_s ==∗
         (⌜head_reducible P_t e_t σ_t⌝ ∗ ∀ e_t' efs_t σ_t', ⌜head_step P_t e_t σ_t e_t' σ_t' efs_t⌝ ==∗
-          ⌜efs_t = []⌝ ∗ state_interp P_t σ_t' P_s σ_s ∗ target_red e_t' Ψ)) -∗
+          ⌜efs_t = []⌝ ∗ state_interp P_t σ_t' P_s σ_s T_s ∗ target_red e_t' Ψ)) -∗
       target_red e_t Ψ.
   Proof.
-    iIntros "Htarget". iApply target_red_step. iIntros (????) "Hstate".
+    iIntros "Htarget". iApply target_red_step. iIntros (?????) "Hstate".
     iMod ("Htarget" with "Hstate") as "(%Hred & Hstep)". iModIntro.
     iSplitR. { iPureIntro. by apply head_prim_reducible. }
     iIntros (e_t' σ_t' efs_t) "%Hprim". iApply "Hstep".
@@ -300,14 +324,15 @@ Section fix_sim.
 
   (** source eval *)
   Lemma source_red_lift_head_step Ψ e_s :
-   ⊢ (∀ P_s σ_s P_t σ_t,
-       state_interp P_t σ_t P_s σ_s ∗ ⌜¬ reach_stuck P_s e_s σ_s⌝ ==∗ ∃ e_s' σ_s',
+   ⊢ (∀ P_s σ_s P_t σ_t T_s K_s,
+       state_interp P_t σ_t P_s σ_s T_s ∗ ⌜T_s !! π = Some (fill K_s e_s) ∧ pool_safe P_s T_s σ_s⌝
+        ==∗ ∃ e_s' σ_s',
           ⌜head_step P_s e_s σ_s e_s' σ_s' []⌝ ∗
-          |==> state_interp P_t σ_t P_s σ_s' ∗ source_red e_s' Ψ) -∗
-      source_red e_s Ψ.
+          |==> state_interp P_t σ_t P_s σ_s' (<[π:=K_s e_s']> T_s) ∗ source_red e_s' π Ψ) -∗
+      source_red e_s π Ψ.
   Proof.
     iIntros "Hsource". iApply source_red_step.
-    iIntros (????) "[Hstate %Hnreach]".
+    iIntros (??????) "[Hstate %Hnreach]".
     iMod ("Hsource" with "[$Hstate//]") as (e_s' σ_s') "[% >Hstate]".
     iModIntro. iExists e_s', σ_s'. iFrame. iPureIntro. by apply head_prim_step.
   Qed.
@@ -316,13 +341,14 @@ Section fix_sim.
   Lemma sim_lift_call Φ fn v_t v_s :
     Ω v_t v_s -∗
     (∀ v_t v_s, Ω v_t v_s -∗ Φ (of_val v_t) (of_val v_s)) -∗
-    (of_call fn v_t) ⪯{Ω} (of_call fn v_s) [{ Φ }].
+    (of_call fn v_t) ⪯{π, Ω} (of_call fn v_s) [{ Φ }].
   Proof.
     iIntros "Hom Hv".
-    rewrite sim_expr_unfold. iIntros (????) "[? ?]". iModIntro. iRight; iRight.
+    rewrite sim_expr_unfold. iIntros (??????) "[? [% %]]". iModIntro. iRight; iRight.
     iExists fn, empty_ectx, v_t, empty_ectx, v_s, σ_s.
     rewrite !fill_empty. iFrame.
     iSplitR; first done. iSplitR; first (iPureIntro; constructor).
+    rewrite list_insert_id; [|done]. iFrame.
     iIntros (v_t' v_s') "Hv'". rewrite !fill_empty. iApply sim_expr_base. by iApply "Hv".
   Qed.
 
@@ -339,22 +365,23 @@ Section fix_sim.
      requires to take steps in the beginning, before escaping to the simulation relation again.
   *)
   Lemma sim_lift_coind (inv : expr Λ → expr Λ → PROP) e_t e_s Φ :
-    (□ ∀ e_t e_s P_t P_s σ_t σ_s,
-      inv e_t e_s -∗ state_interp P_t σ_t P_s σ_s ∗ ⌜¬ reach_stuck P_s e_s σ_s⌝ ==∗
+    (□ ∀ e_t e_s P_t P_s σ_t σ_s T_s K_s,
+      inv e_t e_s -∗ state_interp P_t σ_t P_s σ_s T_s ∗ ⌜T_s !! π = Some (fill K_s e_s)
+        ∧ pool_safe P_s T_s σ_s⌝ ==∗
         ⌜reducible P_t e_t σ_t⌝ ∗
         ∀ e_t' efs_t σ_t',
           ⌜prim_step P_t e_t σ_t e_t' σ_t' efs_t⌝ ==∗
           ∃ e_s' σ_s', ⌜efs_t = []⌝ ∗ ⌜prim_step P_s e_s σ_s e_s' σ_s' []⌝ ∗
-            state_interp P_t σ_t' P_s σ_s' ∗
-            e_t' ⪯{Ω} e_s' [{ λ e_t'' e_s'', Φ e_t'' e_s'' ∨ inv e_t'' e_s'' }]) -∗
+            state_interp P_t σ_t' P_s σ_s' (<[π:=K_s e_s']>T_s) ∗
+            e_t' ⪯{π, Ω} e_s' [{ λ e_t'' e_s'', Φ e_t'' e_s'' ∨ inv e_t'' e_s'' }]) -∗
     inv e_t e_s -∗
-    e_t ⪯{Ω} e_s [{ Φ }].
+    e_t ⪯{π, Ω} e_s [{ Φ }].
   Proof.
-    pose (F  := (λ Ψ e_t e_s, (∀ e_t e_s, Φ e_t e_s -∗ Ψ e_t e_s) ∗ inv e_t e_s)%I).
+    pose (F  := (λ Ψ π' e_t e_s, (∀ e_t e_s, Φ e_t e_s -∗ Ψ e_t e_s) ∗ ⌜π = π'⌝ ∗ inv e_t e_s)%I).
     iIntros "#H Inv". iApply (sim_expr_paco _ F).
-    { intros ??? Heq ??; rewrite /F. repeat f_equiv. by apply Heq. }
-    - iModIntro. clear. iIntros (Ψ e_t e_s) "[Himpl Hinv]".
-      rewrite /lock_step. iIntros (p_t σ_t p_s σ_s) "Hs".
+    { intros ??? Heq ???; rewrite /F. repeat f_equiv. by apply Heq. }
+    - iModIntro. clear. iIntros (Ψ π' e_t e_s) "[Himpl [% Hinv]]". subst π'.
+      rewrite /lock_step. iIntros (p_t σ_t p_s σ_s T_s K_s) "Hs".
       iMod ("H" with "Hinv Hs") as "[$ Hcont]".
       iModIntro. iIntros (e_t' σ_t' efs_t Hstep).
       iMod ("Hcont" with "[//]") as (e_s' σ_s') "(H1 & H2 & H3 & H4)".
@@ -362,24 +389,25 @@ Section fix_sim.
       iApply (sim_expr_mono with "[Himpl] H4").
       clear. iIntros (e_t e_s) "[H1|H1]".
       + iRight. by iApply "Himpl".
-      + iLeft. iFrame.
-    - rewrite /F. iFrame. clear. iIntros (e_t e_s) "$".
+      + iLeft. by iFrame.
+    - rewrite /F. iFrame. iSplit; [|done]. clear. iIntros (e_t e_s) "$".
   Qed.
 
   Lemma sim_lift_head_coind (inv : expr Λ → expr Λ → PROP) e_t e_s Φ :
-    (□ ∀ e_t e_s P_t P_s σ_t σ_s,
-      inv e_t e_s -∗ state_interp P_t σ_t P_s σ_s ∗ ⌜¬ reach_stuck P_s e_s σ_s⌝ ==∗
+    (□ ∀ e_t e_s P_t P_s σ_t σ_s T_s K_s,
+      inv e_t e_s -∗ state_interp P_t σ_t P_s σ_s T_s ∗ ⌜T_s !! π = Some (fill K_s e_s)
+        ∧ pool_safe P_s T_s σ_s⌝ ==∗
         ⌜head_reducible P_t e_t σ_t⌝ ∗
         ∀ e_t' efs_t σ_t',
           ⌜head_step P_t e_t σ_t e_t' σ_t' efs_t⌝ ==∗
           ∃ e_s' σ_s', ⌜efs_t = []⌝ ∗ ⌜head_step P_s e_s σ_s e_s' σ_s' []⌝ ∗
-            state_interp P_t σ_t' P_s σ_s' ∗
-            e_t' ⪯{Ω} e_s' [{ λ e_t'' e_s'', Φ e_t'' e_s'' ∨ inv e_t'' e_s'' }]) -∗
+            state_interp P_t σ_t' P_s σ_s' (<[π:=K_s e_s']> T_s) ∗
+            e_t' ⪯{π, Ω} e_s' [{ λ e_t'' e_s'', Φ e_t'' e_s'' ∨ inv e_t'' e_s'' }]) -∗
     inv e_t e_s -∗
-    e_t ⪯{Ω} e_s [{ Φ }].
+    e_t ⪯{π, Ω} e_s [{ Φ }].
   Proof.
     iIntros "#Ha Hinv". iApply (sim_lift_coind with "[] Hinv").
-    iModIntro. iIntros (??????) "Hinv [Hstate %Hnreach]".
+    iModIntro. iIntros (????????) "Hinv [Hstate [% %]]".
     iMod ("Ha" with "Hinv [$Hstate//]") as "[%Hred Hs]". iModIntro.
     iSplitR. { iPureIntro. by apply head_prim_reducible. }
     iIntros (???) "%Hprim". iMod ("Hs" with "[]") as (e_s' σ_s') "(% & %Hhead & Hstate & Hs)".
@@ -388,43 +416,45 @@ Section fix_sim.
   Qed.
 
   Lemma sim_lift_coind' (inv : expr Λ → expr Λ → PROP) e_t e_s Φ :
-    (□ ∀ e_t e_s P_t P_s σ_t σ_s,
-      inv e_t e_s -∗ state_interp P_t σ_t P_s σ_s ∗ ⌜¬ reach_stuck P_s e_s σ_s⌝ ==∗
+    (□ ∀ e_t e_s P_t P_s σ_t σ_s T_s K_s,
+      inv e_t e_s -∗ state_interp P_t σ_t P_s σ_s T_s ∗ ⌜T_s !! π = Some (fill K_s e_s)
+        ∧ pool_safe P_s T_s σ_s⌝ ==∗
         ⌜reducible P_t e_t σ_t⌝ ∗
         ∀ e_t' efs_t σ_t',
           ⌜prim_step P_t e_t σ_t e_t' σ_t' efs_t⌝ ==∗
           ∃ e_s' σ_s', ⌜efs_t = []⌝ ∗ ⌜prim_step P_s e_s σ_s e_s' σ_s' []⌝ ∗
-            state_interp P_t σ_t' P_s σ_s' ∗
+            state_interp P_t σ_t' P_s σ_s' (<[π:=K_s e_s']> T_s) ∗
             (∀ Ψ,
             □ (∀ e_t e_s, inv e_t e_s -∗ Ψ e_t e_s) -∗
             □ (∀ e_t e_s, Φ e_t e_s -∗ Ψ e_t e_s) -∗
-            e_t' ⪯{Ω} e_s' [{ Ψ }])) -∗
+            e_t' ⪯{π, Ω} e_s' [{ Ψ }])) -∗
     inv e_t e_s -∗
-    e_t ⪯{Ω} e_s [{ Φ }].
+    e_t ⪯{π, Ω} e_s [{ Φ }].
   Proof.
     iIntros "#H Inv". iApply (sim_lift_coind with "[H] Inv").
-    iModIntro. iIntros (??????) "Hinv Hs". iMod ("H" with "Hinv Hs") as "[$ Hs]".
+    iModIntro. iIntros (????????) "Hinv Hs". iMod ("H" with "Hinv Hs") as "[$ Hs]".
     iModIntro. iIntros (???) "Hstep". iMod ("Hs" with "Hstep") as (e_s' σ_s') "($ & Hstep & Hsi & Hsim)".
     iExists e_s', σ_s'. iModIntro. iFrame. iApply "Hsim"; eauto.
   Qed.
 
   Lemma sim_lift_head_coind' (inv : expr Λ → expr Λ → PROP) e_t e_s Φ :
-    (□ ∀ e_t e_s P_t P_s σ_t σ_s,
-      inv e_t e_s -∗ state_interp P_t σ_t P_s σ_s ∗ ⌜¬ reach_stuck P_s e_s σ_s⌝ ==∗
+    (□ ∀ e_t e_s P_t P_s σ_t σ_s T_s K_s,
+      inv e_t e_s -∗ state_interp P_t σ_t P_s σ_s T_s ∗ ⌜T_s !! π = Some (fill K_s e_s)
+        ∧ pool_safe P_s T_s σ_s⌝ ==∗
         ⌜head_reducible P_t e_t σ_t⌝ ∗
         ∀ e_t' efs_t σ_t',
           ⌜head_step P_t e_t σ_t e_t' σ_t' efs_t⌝ ==∗
           ∃ e_s' σ_s', ⌜efs_t = []⌝ ∗ ⌜head_step P_s e_s σ_s e_s' σ_s' []⌝ ∗
-            state_interp P_t σ_t' P_s σ_s' ∗
+            state_interp P_t σ_t' P_s σ_s' (<[π:=K_s e_s']>T_s) ∗
             (∀ Ψ,
             □ (∀ e_t e_s, inv e_t e_s -∗ Ψ e_t e_s) -∗
             □ (∀ e_t e_s, Φ e_t e_s -∗ Ψ e_t e_s) -∗
-            e_t' ⪯{Ω} e_s' [{ Ψ }])) -∗
+            e_t' ⪯{π, Ω} e_s' [{ Ψ }])) -∗
     inv e_t e_s -∗
-    e_t ⪯{Ω} e_s [{ Φ }].
+    e_t ⪯{π, Ω} e_s [{ Φ }].
   Proof.
     iIntros "#H Inv". iApply (sim_lift_head_coind with "[H] Inv").
-    iModIntro. iIntros (??????) "Hinv Hs". iMod ("H" with "Hinv Hs") as "[$ Hs]".
+    iModIntro. iIntros (????????) "Hinv Hs". iMod ("H" with "Hinv Hs") as "[$ Hs]".
     iModIntro. iIntros (???) "Hstep". iMod ("Hs" with "Hstep") as (e_s' σ_s') "($ & Hstep & Hsi & Hsim)".
     iExists e_s', σ_s'. iModIntro. iFrame. iApply "Hsim"; eauto.
   Qed.
